src/Address.v
@@ -1,4 +1,5 @@
 Require Export SpecCert.Address.AddressSpace.
 Require Export SpecCert.Address.Address.
+Require Export SpecCert.Address.LogicalAddress.
 Require Export SpecCert.Address.PhysicalAddress.
 Require Export SpecCert.Address.HardwareAddress.
