src/Address/PhysicalAddress.v
@@ -15,70 +15,20 @@ Require Import SpecCert.Equality.
 Inductive MemoryMap :=
 | mm: MemoryMap.
 
-Lemma mm_singleton: forall m m': MemoryMap, m = m'.
-Proof.
-  induction m; induction m'; reflexivity.
-Qed.
-
-Definition mm_eq
-           (m m': MemoryMap)
-  : Prop :=
-  m = m'.
-
-Definition mm_eq_dec
-           (m m': MemoryMap)
-  : {mm_eq m m'}+{~ mm_eq m m'}.
-  left.
-  apply mm_singleton.
-Defined.
-
-Lemma mm_eq_refl
-      (m: MemoryMap)
-  : mm_eq m m.
-Proof.
-  unfold mm_eq; auto.
-Qed.
-
-Lemma mm_eq_sym
+Lemma mm_singleton
       (m m': MemoryMap)
-  : mm_eq m m' -> mm_eq m' m.
+  : m = m'.
 Proof.
-  unfold mm_eq; auto.
+  induction m; induction m'.
+  reflexivity.
 Qed.
 
-Lemma mm_eq_trans
-      (m m' m'': MemoryMap)
-  : mm_eq m m'
-    -> mm_eq m' m''
-    -> mm_eq m m''.
-Proof.
-  rewrite (mm_singleton m' m); rewrite (mm_singleton m'' m).
-  trivial.
-Qed.
+Instance mmSingleton
+  : Singleton MemoryMap := { singleton := mm_singleton }.
 
-Lemma mm_eq_eq
-      (m m': MemoryMap)
-  : mm_eq m m' -> m = m'.
-unfold mm_eq; auto.
-Qed.
-
-Lemma eq_mm_eq
-      (m m': MemoryMap)
-  : m = m' -> mm_eq m m'.
-Proof.
-  intro Heq.
-  apply mm_singleton.
-Qed.
-
-Instance memoryMapEq : Eq MemoryMap :=
-  { eq       := mm_eq
-  ; eq_refl  := mm_eq_refl
-  ; eq_sym   := mm_eq_sym
-  ; eq_trans := mm_eq_trans
-  ; eq_dec   := mm_eq_dec
-  ; eq_equal := mm_eq_eq
-  ; equal_eq := eq_mm_eq
-  }.
+Instance memoryMapEq
+  : Eq MemoryMap
+  := singletonEq MemoryMap.
 
 Definition PhysicalAddress := Address MemoryMap.
 
